---
title: "Tarea 7"
author: "Oscar Gerardo Hernández Martínez"
date: "25/9/2019"
output: pdf_document
---

$$x^2y'' + 2xy' -2y = 0$$
$$y_1 = x$$
$$y_1 = x, \ \ \ \ \ \ \ y'_1 = 1, \ \ \ \ \ \ \ y''_1 = 0$$

> Sutitución: $x^2(0) + 2x(1) - 2x = 0 \checkmark$

> Encontramos $u$

$$y'' + \frac{2x}{x^2}y' - \frac{2y}{x^2} = 0 \ \ \rightarrow \ \ y'' + \frac{2y'}{x} - \frac{2y}{x^2} = 0$$
$$P(x) = \frac{2}{x}, \ \ \ \ \ Q(x) = -\frac{2}{x^2}$$
$$u = \int \frac{e^{-\int \frac{2}{x}dx}}{(x)^2}dx \ \rightarrow \ \int \frac{e^{-ln|x|}}{x^2}dx \ \rightarrow \ \int \frac{x^{-2}}{x^2}dx$$
$$u = -\frac{1}{3}x^{-3}, \ \ \ \ \ \ y_2=uy_1 \ \rightarrow \ y_2 = -\frac{1}{3}x^{-3}x$$
$$\therefore y_2 = -\frac{1}{3}x^{-2}$$

> Solución general 

$$y = C_1x - C_2\frac{1}{3}x^{-2} \ \rightarrow \ y = C_1x + C_2x^{-2}$$